restructuring monotone refs

ulib/FStar.Monotonic.RRef.fst
@@ -6,8 +6,8 @@ open FStar.HyperHeap
 open FStar.HyperStack
 open FStar.HST
 
+module HH = FStar.HyperHeap
 module HS = FStar.HyperStack
-module HST = FStar.HST
 
 let reln (a:Type) = a -> a -> Type
 
@@ -15,8 +15,10 @@ let monotonic (a:Type) (b:reln a) =
   (forall x. b x x)                             (* reflexive *)
   /\ (forall x y z. b x y /\ b y z ==> b x z)   (* transitive *)
 
-//adding eternal region for now, since it is used with ralloc
-type rid = r:rid{HS.is_eternal_region r}
+(*
+ * AR: adding is_eternal_region refinement, since mrefs are allocated using ralloc
+ *)
+type rid = r:HH.rid{is_eternal_region r}
 
 abstract type m_rref (r:rid) (a:Type) (b:reln a) = x:HS.ref a{x.id = r}
 
@@ -26,23 +28,38 @@ let haseq_m_rref (r:rid) (a:Type) (b:reln a)
 	    [SMTPat (hasEq (m_rref r a b))]
     = ()
 
-val as_rref: #r:rid -> #a:Type -> #b:reln a -> m_rref r a b -> GTot (rref r a)
-let as_rref #r #a #b x = x.ref
+(* val as_rref: #r:rid -> #a:Type -> #b:reln a -> m_rref r a b -> GTot (rref r a) *)
+(* let as_rref #r #a #b x = x *)
 
-val as_reference: #r:rid -> #a:Type -> #b:reln a -> m_rref r a b  -> GTot (ref a)
-let as_reference #r #a #b x = x
+(*
+ * AR: the refinement is important here, for as_rref rid was part of the type index
+ *)
+val as_hsref: #r:rid -> #a:Type -> #b:reln a -> m_rref r a b -> GTot (x:HS.ref a{x.id = r})
+let as_hsref #r #a #b x = x
 
-val m_contains : #r:rid -> #a:Type -> #b:reln a -> mr:m_rref r a b -> m:t -> GTot bool
-let m_contains #r #a #b mr m = HyperHeap.contains_ref (as_rref mr) m
+(* val m_contains : #r:rid -> #a:Type -> #b:reln a -> mr:m_rref r a b -> m:t -> GTot bool *)
+(* let m_contains #r #a #b mr m = HyperHeap.contains_ref (as_rref mr) m *)
 
-let m_fresh (#r:rid) (#a:Type) (#b:reln a) (mr:m_rref r a b) (m0:t) (m1:t) : GTot Type0 =
-  HyperHeap.fresh_rref (as_rref mr) m0 m1
+let m_contains (#r:rid) (#a:Type) (#b:reln a) (mr:m_rref r a b) (m:mem) = HS.contains m (as_hsref mr)
 
-val m_sel: #r:rid -> #a:Type -> #b:reln a -> h:t -> m_rref r a b -> GTot a
-let m_sel #r #a #b h m = HyperHeap.sel h (as_rref m)
+(* let m_fresh (#r:rid) (#a:Type) (#b:reln a) (mr:m_rref r a b) (m0:t) (m1:t) : GTot Type0 = *)
+(*   HyperHeap.fresh_rref (as_rref mr) m0 m1 *)
 
-val m_upd: #r:rid -> #a:Type -> #b:reln a -> h:t -> m_rref r a b -> a -> GTot t
-let m_upd #r #a #b h m v = HyperHeap.upd h (as_rref m) v
+let m_fresh (#r:rid) (#a:Type) (#b:reln a) (mr:m_rref r a b) (m0:mem) (m1:mem) : GTot Type0 =
+  let hsref = as_hsref mr in
+  HyperHeap.fresh_rref hsref.ref m0.h m1.h
+
+(* val m_sel: #r:rid -> #a:Type -> #b:reln a -> h:t -> m_rref r a b -> GTot a *)
+(* let m_sel #r #a #b h m = HyperHeap.sel h (as_rref m) *)
+
+val m_sel: #r:rid -> #a:Type -> #b:reln a -> h:mem -> m_rref r a b -> GTot a
+let m_sel #r #a #b h m = HS.sel h (as_hsref m)
+
+(* val m_upd: #r:rid -> #a:Type -> #b:reln a -> h:t -> m_rref r a b -> a -> GTot t *)
+(* let m_upd #r #a #b h m v = HyperHeap.upd h (as_rref m) v *)
+
+val m_upd: #r:rid -> #a:Type -> #b:reln a -> h:mem{live_region h r} -> m_rref r a b -> a -> GTot mem
+let m_upd #r #a #b h m v = HS.upd h (as_hsref m) v
 
 val m_alloc: #a:Type
           -> #b:reln a
@@ -50,16 +67,16 @@ val m_alloc: #a:Type
             -> init:a
             -> ST (m_rref r a b)
 		(requires (fun _ -> monotonic a b))
-		(ensures (fun h0 (m:m_rref r a b) h1 -> ralloc_post r init h0 (as_reference m) h1))
-let m_alloc #a #b r init = ralloc r init
+		(ensures (fun h0 (m:m_rref r a b) h1 -> ralloc_post r init h0 (as_hsref m) h1))
+let m_alloc #a #b r init = HST.ralloc r init
 
 val m_read:#r:rid 
        -> #a:Type
        -> #b:reln a
        -> x:m_rref r a b
        -> ST a
-            (requires (fun h -> h `contains` (as_reference x)))
-            (ensures (deref_post (as_reference x)))
+            (requires (fun h -> h `contains` (as_hsref x)))
+            (ensures (deref_post (as_hsref x)))
 let m_read #r #a #b x = !x
 
 val m_write:#r:rid 
@@ -68,53 +85,54 @@ val m_write:#r:rid
         -> x:m_rref r a b
         -> v:a
         -> ST unit
-              (requires (fun h0 -> h0 `contains` (as_reference x) /\ b (m_sel h0.h x) v))
-              (ensures (assign_post (as_reference x) v))
+              (requires (fun h0 -> h0 `contains` (as_hsref x) /\ b (m_sel h0 x) v))
+              (ensures (assign_post (as_hsref x) v))
 let m_write #r #a #b x v = x := v
 
-inline type stable_on_t (#i:rid) (#a:Type) (#b:reln a) (r:m_rref i a b) (p:(t -> GTot Type0)) =
+(*
+ * AR: adding live_region to HS.m_sel breaks this, there needs to be live_region here too.
+ *)
+inline type stable_on_t (#i:rid) (#a:Type) (#b:reln a) (r:m_rref i a b) (p:(mem -> GTot Type0)) =
   forall h0 h1. p h0 /\ b (m_sel h0 r) (m_sel h1 r) ==> p h1
-abstract type witnessed (p:(t -> GTot Type0)) = True
+abstract type witnessed (p:(mem -> GTot Type0)) = True
 
 val witness: #r:rid
           -> #a:Type
           -> #b:reln a
           -> m:m_rref r a b
-          -> p:(t -> GTot Type0)
+          -> p:(mem -> GTot Type0)
           -> ST unit
-                (requires (fun h0 -> p h0.h /\ stable_on_t m p))
+                (requires (fun h0 -> p h0 /\ stable_on_t m p))
                 (ensures (fun h0 _ h1 -> h0==h1 /\ witnessed p))
 let witness #r #a #b m p = ()
 
-assume val weaken_witness : p:(t -> GTot Type0) 
-			  -> q:(t -> GTot Type0) 
+assume val weaken_witness : p:(mem -> GTot Type0) 
+			  -> q:(mem -> GTot Type0) 
 			  -> Lemma
   ((forall h. p h ==> q h) /\ witnessed p ==> witnessed q)
 
-val testify: p:(t -> GTot Type0)
+val testify: p:(mem -> GTot Type0)
           -> ST unit
                (requires (fun _ ->  witnessed p))
-               (ensures (fun h0 _ h1 -> h0==h1 /\ p h1.h))
+               (ensures (fun h0 _ h1 -> h0==h1 /\ p h1))
 let testify p = admit() //intentionally admitted
 
 
-val testify_forall: #a:Type -> #p:(a -> t -> Type0) 
+val testify_forall: #a:Type -> #p:(a -> mem -> Type0) 
        -> $s:squash (forall (x:a). witnessed (p x)) 
        -> ST unit
   (requires (fun h -> True))
-  (ensures (fun h0 _ h1 -> h0==h1 /\ (forall (x:a). p x h1.h)))
+  (ensures (fun h0 _ h1 -> h0==h1 /\ (forall (x:a). p x h1)))
 let testify_forall #a #p $s = admit() //intentionally admitted
-
 
 val m_recall: #r:rid -> #a:Type -> #b:reln a 
             -> m:m_rref r a b
 	    -> ST unit 
 	      (requires (fun h -> True))
-	      (ensures (fun h0 _ h1 -> h0==h1 /\ h1 `contains` (as_reference m)))
+	      (ensures (fun h0 _ h1 -> h0==h1 /\ m_contains m h1))
 let m_recall #r #a #b m = recall m
 
-
-let rid_exists (r:rid) (h:t) = b2t(Map.contains h r)
+let rid_exists (r:rid) (h:mem) = b2t(Map.contains h.h r)
 // ex_rid: The type of a region id that is known to exist now and for ever more
 type ex_rid = r:rid{witnessed (rid_exists r)}
 
